partial stuff

coq/QLearn/Tsitsiklis.v
@@ -5301,16 +5301,6 @@ Section MDP.
     fun sa => FiniteExpectation prts (cost sa) +
               β * (FiniteExpectation prts (fun ω => qlearn_Qmin Q (next_state sa ω))).
 
-
-  Instance rv_qmin1 (Q : Ts -> Rfct (sigT M.(act)))
-           (rvQ : forall sa, RandomVariable dom borel_sa (fun ω => Q ω sa))
-           (sa : (sigT M.(act))) :
-    RandomVariable dom borel_sa 
-                   (fun ω : Ts => qlearn_Qmin (Q ω) (next_state sa ω)).
-  Proof.
-  Admitted.
-
-
   Instance rvs_Rmin_list (rvs : list (Ts -> R))
                           {rv_rvs : List.Forall (RandomVariable dom borel_sa) rvs} :
     RandomVariable dom borel_sa (fun ω : Ts => Rmin_list (map (fun x => x ω) rvs)).
@@ -5391,6 +5381,40 @@ Section MDP.
       now destruct H as [? [??]]; subst.
   Qed.      
 
+  Instance rv_Rmin_all (Q : Ts -> Rfct (sigT M.(act)))
+    (isrvQ : forall sa, RandomVariable dom borel_sa (fun ω => Q ω sa)) :
+    RandomVariable dom borel_sa (fun ω : Ts => Rmin_all (Q ω)).
+  Proof.
+    unfold Rmin_all.
+    match_destr.
+    generalize (@rvs_Rmin_list ((map (fun (s : sigT (act M)) ω => Q ω s) fin_elms))); intros HH.
+    cut_to HH.
+    - revert HH.
+      apply RandomVariable_proper; try easy.
+      intros ?.
+      now rewrite map_map.
+    - apply Forall_forall; intros.
+      apply in_map_iff in H.
+      now destruct H as [? [??]]; subst.
+  Qed.      
+
+  Instance rv_Rmax_all (Q : Ts -> Rfct (sigT M.(act)))
+    (isrvQ : forall sa, RandomVariable dom borel_sa (fun ω => Q ω sa)) :
+    RandomVariable dom borel_sa (fun ω : Ts => Rmax_all (Q ω)).
+  Proof.
+    unfold Rmax_all.
+    match_destr.
+    generalize (@rvs_Rmax_list ((map (fun (s : sigT (act M)) ω => Q ω s) fin_elms))); intros HH.
+    cut_to HH.
+    - revert HH.
+      apply RandomVariable_proper; try easy.
+      intros ?.
+      now rewrite map_map.
+    - apply Forall_forall; intros.
+      apply in_map_iff in H.
+      now destruct H as [? [??]]; subst.
+  Qed.      
+
   Instance isfe_Rmax_all (Q : Ts -> Rfct (sigT M.(act)))
     (isrvQ : forall sa, RandomVariable dom borel_sa (fun ω => Q ω sa))
     (isfeQ : forall sa, IsFiniteExpectation prts (fun ω => Q ω sa)) :
@@ -5411,6 +5435,51 @@ Section MDP.
       apply in_map_iff in H.
       now destruct H as [? [??]]; subst.
   Qed.      
+
+  Definition event_st_eq (rvs : Ts -> M.(state)) 
+             (s0 : M.(state)) : event dom.
+  Admitted.
+
+  Lemma qlearn_Qmin_Rmin_indicator (Q : Ts -> Rfct (sigT M.(act))) :
+    forall sa,
+      rv_eq
+        (fun ω : Ts => qlearn_Qmin (Q ω) (next_state sa ω))
+        (fun ω => Rmin_list
+                    (map (fun sa0 =>
+                            rvmult (fun ω => Q ω sa0)
+                                   (EventIndicator 
+                                      (classic_dec
+                                         (event_st_eq 
+                                            (next_state sa)
+                                            (projT1 sa0)))) ω)
+                         fin_elms)).
+    Proof.
+      Admitted.
+
+  Instance rv_qmin1 (Q : Ts -> Rfct (sigT M.(act)))
+           (rvQ : forall sa, RandomVariable dom borel_sa (fun ω => Q ω sa))
+           (sa : (sigT M.(act))) :
+    RandomVariable dom borel_sa 
+                   (fun ω : Ts => qlearn_Qmin (Q ω) (next_state sa ω)).
+  Proof.
+    assert (RandomVariable 
+              dom borel_sa
+              (fun ω => Rmin_list
+                          (map (fun sa0 =>
+                                  rvmult (fun ω => Q ω sa0)
+                                         (EventIndicator 
+                                            (classic_dec
+                                               (event_st_eq 
+                                                  (next_state sa)
+                                                  (projT1 sa0)))) ω)
+                               fin_elms))).
+    {
+      admit.
+    }
+    revert H.
+    apply RandomVariable_proper; try easy.
+    apply qlearn_Qmin_Rmin_indicator.
+  Admitted.
 
   Instance isfe_qmin1 (Q : Ts -> Rfct (sigT M.(act)))
     (isrvQ : forall sa, RandomVariable dom borel_sa (fun ω => Q ω sa))
